GeneralizedRewriting/EautoHints.lean
@@ -1,0 +1,63 @@
+
+/-
+## Hint databases and hint declaration
+-/
+
+import Lean
+open Lean Meta
+
+namespace Eauto
+
+inductive Hint where
+  | Constant (n: Name) (expr: Expr) (type: Expr)
+  | Extern (term: Term) (tactic: TSyntax `tactic) (cost: Nat)
+
+instance : ToMessageData Hint where
+  toMessageData
+    | .Constant n _ type => m!"{n}: {type}"
+    | .Extern term tactic cost => m!"Extern {cost}: {term} => {tactic}"
+
+structure HintDescr where
+  databaseName: Name
+  hint: Hint
+
+structure HintDB where
+  name: Name
+  hints: Array Hint
+
+instance: ToMessageData HintDB where
+  toMessageData db :=
+    m!"in database {db.name}:\n  " ++
+    MessageData.joinSep (db.hints.toList.map toMessageData) (.ofFormat "\n  ")
+
+abbrev EautoDB := Array HintDB
+
+def EautoDB.addHint (dbs: EautoDB) (h: HintDescr): EautoDB :=
+  match dbs.findIdx? (fun db => db.name = h.databaseName) with
+  | some i =>
+      dbs.modify i (fun db => { db with hints := db.hints.push h.hint })
+  | none =>
+      dbs.push ({ name := h.databaseName, hints := #[h.hint] })
+
+def EautoDB.importHints (aah: Array (Array HintDescr)): ImportM EautoDB :=
+  return aah.foldl (fun dbs ah => ah.foldl EautoDB.addHint dbs) #[]
+
+def EautoDB.exportHints (dbs: EautoDB): Array HintDescr := Id.run do
+  let mut ah := #[]
+  for db in dbs do
+    for hint in db.hints do
+      ah := ah.push { databaseName := db.name, hint := hint }
+  return ah
+
+def EautoDB.getDB (dbs: EautoDB) (name: Name): CoreM HintDB :=
+  match dbs.find? (fun db => db.name = name) with
+  | some db => return db
+  | none => throwError m!"no eauto database called {name}"
+
+initialize eautoDatabaseExtension: PersistentEnvExtension HintDescr HintDescr EautoDB ←
+  registerPersistentEnvExtension {
+    mkInitial := return #[],
+    addImportedFn := EautoDB.importHints,
+    addEntryFn := EautoDB.addHint,
+    exportEntriesFn := EautoDB.exportHints,
+  }
