GeneralizedRewriting/TestsEauto.lean
@@ -3,6 +3,8 @@
 -/
 
 import GeneralizedRewriting.Eauto
+import GeneralizedRewriting.Defs
+
 set_option trace.Meta.Tactic.eauto true
 set_option trace.Meta.Tactic.eauto.hints true
 
@@ -26,6 +28,63 @@ example (Pα: α → Prop) (f: forall a, Pα a → β) (a: α) (ha: Pα a): β :
 
 -- Backtracking example; using ha₁ first which is incorrect
 example (P₁ P₂: α → Prop) (f: forall (a: α), P₁ a → P₂ a → β)
-        (a: α) (ha₁: P₁ a)
+        (a: α) (_: P₁ a)
         (a': α) (ha'₁: P₁ a') (ha'₂: P₂ a'): β := by
   eauto
+
+--== Typeclass resolution cases (on local context) ==--
+
+-- Simplest grewrite case
+example {α β: Type} {Rα: relation α} {Pα: α → Prop}
+  (h₁: Proper (Rα ==> Iff) Pα)
+  (I₁: forall {T: Type} {R: relation T}, Subrel R R)
+  (I₂: Subrel Iff (flip impl))
+  (goal: forall (R₁: relation (α → Prop)) (R₂: relation Prop),
+     Proper R₁ Pα →
+     Subrel R₁ (Rα ==> R₂) →
+     Subrel R₂ (flip impl) → β): β := by
+  eauto
+
+-- Now we force the use of Subrel_respectful, which has instance arguments
+example {α β: Type} {Rα: relation α} {Pα: α → Prop}
+  (h₁: Proper (Rα ==> Iff) Pα)
+  (I₁: Subrel Rα Rα)
+  (I₂: Subrel (flip impl) (flip impl))
+  (I₃: Subrel Iff (flip impl))
+  (goal: forall (R₁: relation (α → Prop)) (R₂: relation Prop),
+     Proper R₁ Pα →
+     Subrel R₁ (Rα ==> R₂) →
+     Subrel R₂ (flip impl) → β): β := by
+  have h := @Subrel_respectful
+  typeclasses_eauto
+
+-- Then we start to introduce generic instances
+example {α β: Type} {Rα: relation α} {Pα: α → Prop}
+  (h₁: Proper (Rα ==> Iff) Pα)
+  (goal: forall (R₁: relation (α → Prop)) (R₂: relation Prop),
+     Proper R₁ Pα →
+     Subrel R₁ (Rα ==> R₂) →
+     Subrel R₂ (flip impl) → β): β := by
+  have h₁ := @Subrel_respectful
+  have h₂ := @Reflexive_Subrel
+  have h₃ := @Reflexive.refl
+  have h₄ := @Subrel_Iff_flip_impl
+  typeclasses_eauto
+
+--== Typeclass resolution cases (on database) ==--
+
+eauto_hint Subrel_respectful: test_eauto
+eauto_hint Reflexive.refl: test_eauto
+eauto_hint Reflexive_Subrel: test_eauto
+eauto_hint Subrel_Iff_flip_impl: test_eauto
+
+#print_eauto_db
+
+-- Only locally-relevant hypotheses in context here
+example {α β: Type _} {Rα: relation α} {Pα: α → Prop}
+  (h₁: Proper (Rα ==> Iff) Pα)
+  (goal: forall (R₁: relation (α → Prop)) (R₂: relation Prop),
+     Proper R₁ Pα →
+     Subrel R₁ (Rα ==> R₂) →
+     Subrel R₂ (flip impl) → β): β := by
+  typeclasses_eauto with test_eauto
